Source/Examples/Factorial.v
@@ -8,23 +8,23 @@ Import Source.
 
 Definition factorial : program := {|
   prog_interface :=
-    mkfmap [(1, {| Component.import := fset [(2, 1)];
-                   Component.export := fset [] |});
+    mkfmap [(Component.main,
+             {| Component.import := fset [(2, 1)];
+                Component.export := fset [] |});
             (2, {| Component.import := fset [];
                    Component.export := fset [1] |})];
   prog_buffers :=
-    mkfmap [(1, inl 1); (2, inl 1)];
+    mkfmap [(Component.main, inl 1); (2, inl 1)];
   prog_procedures :=
     mkfmap [
-      (1, mkfmap [
-        (1, E_call 2 1 (E_val (Int 6)))]);
+      (Component.main, mkfmap [
+        (Procedure.main, E_call 2 1 (E_val (Int 6)))]);
       (2, mkfmap [
         (1, E_if (E_binop Leq (E_deref E_local) (E_val (Int 1)))
                  (E_val (Int 1))
                  (E_binop Mul
                           (E_deref E_local)
-                          (E_call 2 1 (E_binop Minus (E_deref E_local) (E_val (Int 1))))))])];
-  prog_main := Some (1, 1)
+                          (E_call 2 1 (E_binop Minus (E_deref E_local) (E_val (Int 1))))))])]
 |}.
 
 Definition fuel := 1000.
