Source/Examples/NestedCalls.v
@@ -8,21 +8,21 @@ Import Source.
 
 Definition nested_calls : program := {|
   prog_interface :=
-    mkfmap [(1, {| Component.import := fset [(2, 1)];
+    mkfmap [(Component.main,
+                {| Component.import := fset [(2, 1)];
                    Component.export := fset [2] |});
-            (2, {| Component.import := fset [(1, 2)];
+            (2, {| Component.import := fset [(Component.main, 2)];
                    Component.export := fset [1] |})];
   prog_buffers :=
-    mkfmap [(1, inl 1); (2, inl 1)];
+    mkfmap [(Component.main, inl 1); (2, inl 1)];
   prog_procedures :=
     mkfmap [
-      (1, mkfmap [
-        (1, E_binop Add (E_val (Int 1)) (E_call 2 1 (E_val (Int 1))));
+      (Component.main, mkfmap [
+        (Procedure.main, E_binop Add (E_val (Int 1)) (E_call 2 1 (E_val (Int 1))));
         (2, E_deref E_local)]);
       (2, mkfmap [
         (1, E_binop Add (E_deref E_local) (E_call 2 2 (E_deref E_local)));
-        (2, E_binop Add (E_deref E_local) (E_call 1 2 (E_deref E_local)))])];
-  prog_main := Some (1, 1)
+        (2, E_binop Add (E_deref E_local) (E_call Component.main 2 (E_deref E_local)))])]
 |}.
 
 Definition fuel := 1000.
